Implement MonadError for StateT

theories/Monads/State.v
@@ -1,6 +1,8 @@
+(** * The state monad transformer *)
+
 From Coq Require Import FunctionalExtensionality.
 
-From mtl.Classes Require Import Monad Trans State.
+From mtl.Classes Require Import All.
 From mtl.Monads Require Import Identity.
 
 Implicit Types s : Type.
@@ -12,31 +14,53 @@ Record StateT s m (a : Type) : Type :=
 Arguments MkStateT {s m a} _.
 Arguments runStateT {s m a} _.
 
-Instance Monad_StateT s m `{Monad m} : Monad (StateT s m) :=
+Definition State s : Type -> Type := StateT s Identity.
+
+(** ** Instances *)
+
+Instance Monad_StateT {s m} `{Monad m} : Monad (StateT s m) :=
   {| pure _ x := MkStateT (fun z => pure (x, z))
    ; bind _ _ u k := MkStateT (fun z =>
      runStateT u z >>= fun '(x, z1) =>
      runStateT (k x) z1)
   |}.
 
-Instance MonadTrans_StateT s : MonadTrans (StateT s) :=
+Instance MonadTrans_StateT {s} : MonadTrans (StateT s) :=
   {| lift _ _ _ u := MkStateT (fun z => u >>= fun x => pure (x, z))
   |}.
 
-Instance MonadState_StateT s m `{Monad m} : MonadState s (StateT s m) :=
+Instance MonadState_StateT {s m} `{Monad m} : MonadState s (StateT s m) :=
   {| get := MkStateT (fun z => pure (z, z))
    ; put z := MkStateT (fun _ => pure (tt, z))
   |}.
 
-Definition State s : Type -> Type := StateT s Identity.
+Instance MonadError_StateT {e s m} `{Monad m} `{MonadError e m} :
+  MonadError e (StateT s m) :=
+  {| throwError _ err := MkStateT (fun _ => throwError err)
+   ; catchError _ u h := MkStateT (fun z =>
+       catchError (runStateT u z) (fun err => runStateT (h err) z))
+  |}.
 
-Lemma injective_runStateT s m a (u v : StateT s m a) :
+(** Interestingly, there is another lawful instance of [MonadError] for [MonadState],
+    which relies on the ability to throw an exception together with the current state. *)
+Definition MonadError_StateT_recoverable {e s m} `{Monad m} `{MonadError (e * s) m} :
+  MonadError e (StateT s m) :=
+  {| throwError _ err := MkStateT (fun z => throwError (err, z))
+   ; catchError _ u h := MkStateT (fun z =>
+       catchError (runStateT u z) (fun '(err, z') => runStateT (h err) z'))
+  |}.
+
+(** ** Simple facts *)
+
+Lemma injective_runStateT {s m a} (u v : StateT s m a) :
   runStateT u = runStateT v -> u = v.
 Proof.
   destruct u, v; intros; f_equal; auto.
 Qed.
 
-Instance LawfulMonad_StateT s m `{LawfulMonad m} : LawfulMonad (StateT s m).
+(** ** Laws *)
+
+Instance LawfulMonad_StateT {s m} `{LawfulMonad m} : LawfulMonad (StateT s m).
 Proof.
   split.
   all: intros; apply injective_runStateT, functional_extensionality; intros; cbn.
@@ -48,7 +72,7 @@ Proof.
     f_equal. apply functional_extensionality. intros []. reflexivity.
 Qed.
 
-Instance LawfulMonadTrans_StateT s m : LawfulMonadTrans (StateT s).
+Instance LawfulMonadTrans_StateT {s m} : LawfulMonadTrans (StateT s).
 Proof.
   split.
   all: intros; cbn; f_equal; apply functional_extensionality; intros.
@@ -57,9 +81,44 @@ Proof.
     rewrite bind_pure_l. reflexivity.
 Qed.
 
-Instance LawfulMonadState_StateT s m `{LawfulMonad m} : LawfulMonadState s (StateT s m).
+Instance LawfulMonadState_StateT {s m} `{LawfulMonad m} : LawfulMonadState s (StateT s m).
 Proof.
   split.
   all: intros; cbn; apply injective_runStateT, functional_extensionality; cbn; intros.
   all: rewrite ?bind_pure_l; try reflexivity.
+Qed.
+
+Instance LawfulMonadError_StateT {e s m}
+  `{LawfulMonad m} {ME : MonadError e m} {LME : LawfulMonadError e m} :
+  LawfulMonadError e (StateT s m).
+Proof.
+  destruct LME.
+  split; intros; cbn; apply injective_runStateT, functional_extensionality;
+    cbn; intros; auto.
+  - apply catch_throw.
+  - rewrite 2 catch_bind. unfold tryError.
+    rewrite !bind_assoc.
+    f_equal.
+    apply functional_extensionality; intros [ | []]; cbn.
+    all: rewrite bind_pure_l; reflexivity.
+Qed.
+
+Theorem LawfulMonadError_StateT_recoverable {e s m}
+  `{LawfulMonad m} {ME : MonadError (e * s) m} {LME : LawfulMonadError (e * s) m} :
+  @LawfulMonadError e (StateT s m) _ MonadError_StateT_recoverable.
+Proof.
+  destruct LME.
+  split; intros; cbn; apply injective_runStateT, functional_extensionality;
+    cbn; intros; auto.
+  - apply catch_throw.
+  - rewrite catch_catch. f_equal. apply functional_extensionality; intros [].
+    reflexivity.
+  - rewrite 2 catch_bind. unfold tryError.
+    rewrite !bind_assoc.
+    f_equal.
+    apply functional_extensionality; intros [ [] | []]; cbn.
+    all: rewrite bind_pure_l; reflexivity.
+  - transitivity (catchError (runStateT u x) throwError).
+    + f_equal; apply functional_extensionality; intros []; auto.
+    + auto.
 Qed.
